moved in lots of relevant files

galois/crypto/hmac.lean
@@ -1,6 +1,9 @@
 /- This defines an hmac primitive.
  -/
 import galois.word
+import galois.tactic.nat
+import galois.bitvec.join
+import galois.crypto.sha2
 
 namespace crypto
 
@@ -21,3 +24,175 @@ definition hmac {olen : ℕ} -- ^ Output length
   hash (ko ++ (hash (ki ++ msg))^.to_list)
 
 end crypto
+
+namespace hmac
+
+/- hash_algorithm -/
+
+inductive hash_algorithm
+  | sha1      : hash_algorithm
+  | sha2_256  : hash_algorithm
+  | ripemd160 : hash_algorithm
+  | sha2_224  : hash_algorithm
+  | sha2_384  : hash_algorithm
+  | sha2_512  : hash_algorithm
+  | sha3_224  : hash_algorithm
+  | sha3_256  : hash_algorithm
+  | sha3_384  : hash_algorithm
+  | sha3_512  : hash_algorithm
+  | sm3       : hash_algorithm
+
+namespace hash_algorithm
+
+protected def to_string : hash_algorithm → string
+| sha1 := "sha1"
+| sha2_256 := "sha2_256"
+| ripemd160 := "ripemd160"
+| sha2_224 := "sha2_224"
+| sha2_384 := "sha2_384"
+| sha2_512 := "sha2_512"
+| sha3_224 := "sha3_224"
+| sha3_256 := "sha3_256"
+| sha3_384 := "sha3_384"
+| sha3_512 := "sha3_512"
+| sm3      := "sm3"
+
+instance : has_to_string hash_algorithm := ⟨ hash_algorithm.to_string ⟩
+
+/- hash length in bytes -/
+definition hash_length : hash_algorithm → ℕ
+  | sha1      := 20
+  | sha2_256  := 32
+  | ripemd160 := 20
+  | sha2_224  := 28
+  | sha2_384  := 48
+  | sha2_512  := 64
+  | sha3_224  := 28
+  | sha3_256  := 32
+  | sha3_384  := 48
+  | sha3_512  := 64
+  | sm3       := 32
+
+lemma max_hash_length (algo : hash_algorithm) : algo.hash_length ≤ 64 :=
+begin
+  cases algo,
+  all_goals { dunfold hash_length },
+  all_goals { galois.tactic.nat.nat_lit_le },
+end
+
+/- block length in bytes -/
+definition block_length (algo : hash_algorithm) : ℕ :=
+  match algo with
+  | sha1      :=  64
+  | sha2_256  :=  64
+  | ripemd160 :=  64
+  | sha2_224  :=  64
+  | sha2_384  := 128
+  | sha2_512  := 128
+  | sha3_224  := 144
+  | sha3_256  := 136
+  | sha3_384  := 104
+  | sha3_512  :=  72
+  | sm3       :=  64
+  end
+
+definition encode (algo : hash_algorithm) : byte :=
+  match algo with
+  | sha1      := 0x0
+  | sha2_256  := 0x1
+  | ripemd160 := 0x2
+  | sha2_224  := 0x3
+  | sha2_384  := 0x4
+  | sha2_512  := 0x5
+  | sha3_224  := 0x7
+  | sha3_256  := 0x8
+  | sha3_384  := 0x9
+  | sha3_512  := 0xA
+  | sm3       := 0xB
+  end
+
+definition decode (w : byte) : option hash_algorithm :=
+  if w = 0x0 then
+    some sha1
+  else if w = 0x1 then
+    some sha2_256
+  else if w = 0x2 then
+    some ripemd160
+  else if w = 0x3 then
+    some sha2_224
+  else if w = 0x4 then
+    some sha2_384
+  else if w = 0x5 then
+    some sha2_512
+  else if w = 0x7 then
+    some sha3_224
+  else if w = 0x8 then
+    some sha3_256
+  else if w = 0x9 then
+    some sha3_384
+  else if w = 0xA then
+    some sha3_512
+  else if w = 0xB then
+    some sm3
+  else
+    none
+
+@[simp]
+lemma decode_encode (a : hash_algorithm) : decode (encode a) = some a :=
+begin
+  cases a,
+  simp [encode, decode],
+  all_goals {
+    simp [encode, decode],
+    smt_tactic.execute smt_tactic.solve_goals
+  }
+end
+
+instance : decidable_eq hash_algorithm := by tactic.mk_dec_eq_instance
+
+------------------------------------------------------------------------
+-- hash
+
+-- | Helper function to speed up length proofs below
+def to_byte_list (m : ℕ) (v : bitvec (8 * m)) : list byte := cast rfl (@bitvec.split_vector 8 m v)
+
+protected
+lemma length_to_byte_list (m : ℕ) (v : bitvec (8 * m)) : (to_byte_list m v).length = m :=
+vector.length_split_vector _ _
+
+def nat_224_decompose : bitvec 224 → list byte := @to_byte_list 28
+def nat_256_decompose : bitvec 256 → list byte := @to_byte_list 32
+def nat_384_decompose : bitvec 384 → list byte := @to_byte_list 48
+def nat_512_decompose : bitvec 512 → list byte := @to_byte_list 64
+
+definition hash : hash_algorithm → list byte → list byte
+| sha2_256  data := nat_256_decompose (crypto.sha256 data)
+| sha2_224  data := nat_224_decompose (crypto.sha224 data)
+| sha2_384  data := nat_384_decompose (crypto.sha384 data)
+| sha2_512  data := nat_512_decompose (crypto.sha512 data)
+| algo data := list.repeat 0 (algo.hash_length)
+
+theorem length_hash_is_hash_length
+: ∀ (algo : hash_algorithm) (data : list byte),
+    (algo.hash data).length = algo.hash_length
+| sha1      data := list.length_repeat _ _
+| sha2_256  data := hash_algorithm.length_to_byte_list _ _
+| ripemd160 data := list.length_repeat _ _
+| sha2_224  data := hash_algorithm.length_to_byte_list _ _
+| sha2_384  data := hash_algorithm.length_to_byte_list _ _
+| sha2_512  data := hash_algorithm.length_to_byte_list _ _
+| sha3_224  data := list.length_repeat _ _
+| sha3_256  data := list.length_repeat _ _
+| sha3_384  data := list.length_repeat _ _
+| sha3_512  data := list.length_repeat _ _
+| sm3       data := list.length_repeat _ _
+
+-- Hash the data using the given algorithm.
+definition hashv (algo : hash_algorithm) (data : list byte) : vector byte algo.hash_length :=
+  ⟨ hash algo data, length_hash_is_hash_length algo data ⟩
+
+end hash_algorithm
+
+end hmac
+
+
