galois/crypto/merkle/merkle_construction.lean
@@ -1,0 +1,185 @@
+import galois.data.bounded_list
+import galois.list.take_drop_lemmas
+
+universes u v
+
+namespace ksi
+namespace merkle
+
+structure combine_result (Link Data : Type) :=
+(root : Data)
+(left : Link)
+(right : Link)
+
+/-- Operations needed to build a Merkle tree.-/
+structure merkle_ops (Leaf Link Data : Type) :=
+(empty_root : Data)
+(leaf_data : Leaf → Data)
+(apply_link : Link → Data → Data)
+(combine_data : Data -> Data → combine_result Link Data)
+(apply_left_correct
+: ∀(x y : Data), apply_link (combine_data x y).left x = (combine_data x y).root)
+(apply_right_correct
+: ∀(x y : Data), apply_link (combine_data x y).right y = (combine_data x y).root)
+
+section types
+
+parameters {Leaf Link Data : Type}
+parameter (s : merkle_ops Leaf Link Data)
+
+/-- This stores information about a path from a leaf to a root.
+
+ max_req_level bounds the length of the links.
+-/
+structure path (max_req_level : ℕ) (root : Data) :=
+(leaf  : Leaf)
+(links : bounded_list Link max_req_level)
+-- Proof theat the
+(root_valid : links.val.foldr s.apply_link (s.leaf_data leaf) = root)
+
+/-- This represents-/
+structure merkle_result (max_req_level : ℕ) (l : list Leaf) :=
+-- what we are aggregating
+(root : Data)
+-- the paths through the tree to get to this point
+(paths : list (path max_req_level root))
+-- what we have not yet aggregated
+(remaining : list Leaf)
+-- Proof we include all the original paths.
+(paths_valid : paths.map path.leaf ++ remaining = l)
+-- The length of the paths
+(remaining_valid : remaining = l.drop (2^max_req_level))
+
+end types
+
+section merkle
+
+-- This contains the types for the leaves of the tree and link elements
+parameters {Leaf Link Data : Type}
+parameter (ops : merkle_ops Leaf Link Data)
+
+def path.extend_none {n:ℕ} {root : Data} (p : path ops n root)
+: path ops n.succ root :=
+  { links := p.links.extend 1
+  , leaf  := p.leaf
+  , root_valid :=
+    begin
+      cases p,
+      cases links,
+      exact root_valid,
+    end
+  }
+
+theorem path_extend_none (n : ℕ) (root : Data)
+: path.leaf ∘ @path.extend_none n root = path.leaf :=
+begin
+  apply funext,
+  intro p,
+  cases p,
+  simp [function.comp, path.extend_none],
+end
+
+def gpath.extend_sibling (n : ℕ) {r r' : Data}
+    (l : Link)
+    (eq : ops.apply_link l r = r')
+    (p : path ops n r)
+: path ops n.succ r' :=
+{ links := p.links.cons l
+, leaf  := p.leaf
+, root_valid :=
+  begin
+    cases p,
+    cases links,
+    simp [bounded_list.cons, root_valid, eq],
+  end
+}
+
+theorem path_extend_sibling (n : ℕ) (r r' : Data) (l : Link)
+  (eq : ops.apply_link l r = r')
+: path.leaf ∘ @gpath.extend_sibling n r r' l eq = path.leaf :=
+begin
+  apply funext,
+  intro p,
+  cases p,
+  simp [function.comp, gpath.extend_sibling],
+end
+
+def dcases_on {T : Type u} {C : list T → Sort v}
+  (n : list T)
+  (base : n = [] → C [])
+  (ind : Π (h : T) (r : list T), n = h::r → C (h :: r))
+: C n :=
+   @list.cases_on T (λl, n = l → C l) n base ind rfl
+
+def merkle_core
+     : Π (n : ℕ) (e : Leaf) (rest : list Leaf),
+       merkle_result ops n (e::rest)
+| 0 e rest :=
+{ root := ops.leaf_data e
+, paths := [{ leaf := e
+            , links := bounded_list.nil
+            , root_valid := rfl,
+            }]
+, remaining := rest
+, paths_valid := rfl
+, remaining_valid := rfl
+}
+| (nat.succ n) e rest := do
+  let left_result := merkle_core n e rest in
+  @dcases_on _ (λr, merkle_result ops n.succ (e::rest)) left_result.remaining
+    (λ(eq : left_result.remaining = []),
+      { root := left_result.root
+      , paths := left_result.paths.map path.extend_none
+      , remaining := left_result.remaining
+      , paths_valid :=
+        begin
+          simp [path_extend_none, left_result.paths_valid],
+        end
+      , remaining_valid :=
+        begin
+          have h : (2^nat.succ n) = 2^n + 2^n,
+          { simp [nat.pow, nat.succ_mul], },
+          have g := left_result.remaining_valid,
+          rw [h, list.drop_add, ← g, eq, list.drop_nil],
+        end
+      })
+    (λ(e' : Leaf) (rest' : list Leaf) (eq : left_result.remaining = e' :: rest'),
+      let right_result := merkle_core n e' rest' in
+      let z := ops.combine_data left_result.root right_result.root in
+      let l_eq := ops.apply_left_correct left_result.root right_result.root in
+      let r_eq := ops.apply_right_correct left_result.root right_result.root in
+      { root := z.root
+      , paths := left_result.paths.map  (gpath.extend_sibling n z.left  l_eq)
+              ++ right_result.paths.map (gpath.extend_sibling n z.right r_eq)
+      , remaining := right_result.remaining
+      , paths_valid :=
+        begin
+          simp [path_extend_sibling, right_result.paths_valid],
+          rw [← eq],
+          exact left_result.paths_valid,
+        end
+      , remaining_valid :=
+        begin
+          have h : (2^nat.succ n) = 2^n + 2^n,
+          { simp [nat.pow, nat.succ_mul], },
+          rw [h, list.drop_add, ← left_result.remaining_valid, eq],
+          exact right_result.remaining_valid,
+        end
+      })
+
+def merkle
+     : Π (n : ℕ) (l : list Leaf), merkle_result ops n l
+| n [] :=
+{ root := ops.empty_root
+, paths := []
+, remaining := []
+, paths_valid := rfl
+, remaining_valid := by simp [list.drop_nil],
+}
+| n (e::r) := merkle_core n e r
+
+
+end merkle
+
+end merkle
+end ksi
